scheduler_handle → scheduler_context.

theories/examples/fibonacci.v
@@ -53,70 +53,70 @@ Section scheduler_G.
   Context (ws_deques : ws_deques Σ).
 
   #[local] Definition fibonacci_aux : val :=
-    rec: "fibonacci_aux" "n" "hdl" :=
+    rec: "fibonacci_aux" "n" "ctx" :=
       if: "n" ≤ #1 then (
         "n"
       ) else (
-        let: "fut1" := scheduler_async ws_deques "hdl" (λ: "hdl", "fibonacci_aux" ("n" - #1) "hdl") in
-        let: "fut2" := scheduler_async ws_deques "hdl" (λ: "hdl", "fibonacci_aux" ("n" - #2) "hdl") in
-        scheduler_await ws_deques "hdl" "fut1" + scheduler_await ws_deques "hdl" "fut2"
+        let: "fut1" := scheduler_async ws_deques "ctx" (λ: "ctx", "fibonacci_aux" ("n" - #1) "ctx") in
+        let: "fut2" := scheduler_async ws_deques "ctx" (λ: "ctx", "fibonacci_aux" ("n" - #2) "ctx") in
+        scheduler_await ws_deques "ctx" "fut1" + scheduler_await ws_deques "ctx" "fut2"
       ).
   Definition fibonacci : val :=
-    λ: "n" "hdl",
-      scheduler_run ws_deques "hdl" (λ: "hdl", fibonacci_aux "n" "hdl").
+    λ: "n" "ctx",
+      scheduler_run ws_deques "ctx" (λ: "ctx", fibonacci_aux "n" "ctx").
 
-  #[local] Lemma fibonacci_aux_spec n sched hdl :
+  #[local] Lemma fibonacci_aux_spec n sched ctx :
     (0 ≤ n)%Z →
     {{{
       scheduler_inv ws_deques sched ∗
-      scheduler_handle ws_deques sched hdl
+      scheduler_context ws_deques sched ctx
     }}}
-      fibonacci_aux #n hdl
+      fibonacci_aux #n ctx
     {{{
       RET #(fib (Z.to_nat n));
-      scheduler_handle ws_deques sched hdl
+      scheduler_context ws_deques sched ctx
     }}}.
   Proof.
-    iLöb as "HLöb" forall (n hdl).
+    iLöb as "HLöb" forall (n ctx).
 
-    iIntros "%Hn %Φ (#Hsched & Hhdl) HΦ".
+    iIntros "%Hn %Φ (#Hsched & Hctx) HΦ".
 
     wp_rec. wp_pures.
     case_bool_decide as Hcase; wp_pures.
 
     - assert (n = 0 ∨ n = 1) as [-> | ->] by lia; iSteps.
 
-    - wp_smart_apply (scheduler_async_spec _ (λ v1, ⌜v1 = #_⌝)%I with "[$Hsched $Hhdl]") as (fut1) "(Hhdl & #Hfut1)".
-      { clear hdl. iIntros "%hdl Hhdl".
-        wp_smart_apply ("HLöb" with "[] [$Hsched $Hhdl]"); iSteps.
+    - wp_smart_apply (scheduler_async_spec _ (λ v1, ⌜v1 = #_⌝)%I with "[$Hsched $Hctx]") as (fut1) "(Hctx & #Hfut1)".
+      { clear ctx. iIntros "%ctx Hctx".
+        wp_smart_apply ("HLöb" with "[] [$Hsched $Hctx]"); iSteps.
       }
-      wp_smart_apply (scheduler_async_spec _ (λ v2, ⌜v2 = #_⌝)%I with "[$Hsched $Hhdl]") as (fut2) "(Hhdl & #Hfut2)".
-      { clear hdl. iIntros "%hdl Hhdl".
-        wp_smart_apply ("HLöb" with "[] [$Hsched $Hhdl]"); iSteps.
+      wp_smart_apply (scheduler_async_spec _ (λ v2, ⌜v2 = #_⌝)%I with "[$Hsched $Hctx]") as (fut2) "(Hctx & #Hfut2)".
+      { clear ctx. iIntros "%ctx Hctx".
+        wp_smart_apply ("HLöb" with "[] [$Hsched $Hctx]"); iSteps.
       }
-      wp_smart_apply (scheduler_await_spec with "[$Hsched $Hhdl $Hfut2]") as (?) "(Hhdl & ->)".
-      wp_smart_apply (scheduler_await_spec with "[$Hsched $Hhdl $Hfut1]") as (?) "(Hhdl & ->)".
+      wp_smart_apply (scheduler_await_spec with "[$Hsched $Hctx $Hfut2]") as (?) "(Hctx & ->)".
+      wp_smart_apply (scheduler_await_spec with "[$Hsched $Hctx $Hfut1]") as (?) "(Hctx & ->)".
       wp_pures.
       rewrite (fib_spec_Z n) // -Nat2Z.inj_add.
       rewrite decide_False; first lia.
       iSteps.
   Qed.
-  Lemma fibonacci_spec (n : nat) sched hdl :
+  Lemma fibonacci_spec (n : nat) sched ctx :
     {{{
       scheduler_inv ws_deques sched ∗
-      scheduler_handle ws_deques sched hdl
+      scheduler_context ws_deques sched ctx
     }}}
-      fibonacci #n hdl
+      fibonacci #n ctx
     {{{
       RET #(fib n);
-      scheduler_handle ws_deques sched hdl
+      scheduler_context ws_deques sched ctx
     }}}.
   Proof.
-    iIntros "%Φ (#Hsched & Hhdl) HΦ".
+    iIntros "%Φ (#Hsched & Hctx) HΦ".
     wp_rec.
-    wp_smart_apply (scheduler_run_spec _ (λ v, ⌜v = #_⌝)%I with "[$Hsched $Hhdl]") as (?) "(Hhdl & ->)"; last iSteps.
-    clear hdl. iIntros "%hdl Hhdl".
-    wp_smart_apply (fibonacci_aux_spec with "[$Hsched $Hhdl]"); first lia.
+    wp_smart_apply (scheduler_run_spec _ (λ v, ⌜v = #_⌝)%I with "[$Hsched $Hctx]") as (?) "(Hctx & ->)"; last iSteps.
+    clear ctx. iIntros "%ctx Hctx".
+    wp_smart_apply (fibonacci_aux_spec with "[$Hsched $Hctx]"); first lia.
     rewrite Nat2Z.id. iSteps.
   Qed.
 End scheduler_G.
